core/ConcreteHoare.v
@@ -1,16 +1,19 @@
-(* Require Import Poulet4.Typed.
+Require Import Coq.ssr.ssrbool.
+Require Import Poulet4.Typed.
 Require Import Poulet4.Syntax.
 Require Import Poulet4.Semantics.
 Require Import ProD3.core.Coqlib.
 Require Import ProD3.core.Hoare.
 Require Import ProD3.core.AssertionLang.
 Require Import Hammer.Tactics.Tactics.
+Require Import Hammer.Plugin.Hammer.
 
 Section ConcreteHoare.
 
 Context {tags_t: Type} {tags_t_inhabitant : Inhabitant tags_t}.
 Notation Val := (@ValueBase tags_t).
-Notation Lval := (@ValueLvalue tags_t).
+Notation SemLval := (@ValueLvalue tags_t).
+Notation Lval := (@AssertionLang.Lval tags_t).
 
 Notation ident := (P4String.t tags_t).
 Notation path := (list ident).
@@ -26,54 +29,77 @@ Variable inst_m : (@inst_mem tags_t).
 (* Variable this : path. *)
 
 Definition hoare_expr (pre : assertion) (expr : Expression) (v : Val) : Prop :=
-  eval_expr pre expr = Some v.
+  eval_expr ge pre expr = Some v.
 
 Lemma hoare_expr_sound : forall p pre expr v,
+  wellformed pre ->
   hoare_expr pre expr v ->
   Hoare.hoare_expr ge p (to_shallow_assertion p pre) expr v.
-Admitted.
+Proof.
+  unfold Hoare.hoare_expr; intros.
+  eapply eval_expr_sound; eassumption.
+Qed.
 
 Definition hoare_lexpr (p : path) (pre : assertion) (expr : @Expression tags_t) (lv : Lval) : Prop :=
-  True. (* TODO *)
+  eval_lexpr expr = Some lv.
+
+Definition ihoare_lexpr (p : path) (pre : Hoare.assertion) (expr : Expression) (lv : SemLval) :=
+  forall st lv' sig,
+    pre st ->
+    exec_lexpr ge p st expr lv' sig ->
+    sig = SContinue /\ semlval_equivb lv' lv.
 
 Lemma hoare_lexpr_sound : forall p pre expr lv,
   hoare_lexpr p pre expr lv ->
-  Hoare.hoare_lexpr ge p (to_shallow_assertion p pre) expr lv.
-Admitted.
+  ihoare_lexpr p (to_shallow_assertion p pre) expr (lval_to_semlval lv).
+Proof.
+  unfold ihoare_lexpr; intros.
+  eapply eval_lexpr_sound; eassumption.
+Qed.
 
 Definition hoare_write (pre : assertion) (lv : Lval) (v : Val) (post : assertion) : Prop :=
-  True. (* TODO *)
+  is_writable_lval lv pre /\ eval_write pre lv v = post.
 
 Lemma hoare_write_sound : forall p pre lv v post,
+  wellformed pre ->
   hoare_write pre lv v post ->
-  Hoare.hoare_write p (to_shallow_assertion p pre) lv v (to_shallow_assertion p post).
-Admitted.
+  Hoare.hoare_write p (to_shallow_assertion p pre) (lval_to_semlval lv) v (to_shallow_assertion p post).
+Proof.
+  unfold Hoare.hoare_write; intros. destruct H1; subst.
+  eapply eval_write_sound; try eassumption.
+Qed.
 
 Inductive hoare_stmt : path -> assertion -> (@Statement tags_t) -> assertion -> Prop :=
   | hoare_stmt_assignment : forall p pre tags lhs rhs typ post lv v,
       hoare_lexpr p pre lhs lv ->
+      is_valid_field pre lv ->
       hoare_expr pre rhs v ->
       hoare_write pre lv v post ->
       hoare_stmt p pre (MkStatement tags (StatAssignment lhs rhs) typ) post.
 
 Lemma hoare_stmt_sound : forall p pre stmt post,
+  wellformed pre ->
   hoare_stmt p pre stmt post ->
   Hoare.hoare_stmt ge inst_m p (to_shallow_assertion p pre) stmt (to_shallow_assertion p post).
 Proof.
-  intros * H_hoare_stmt.
+  intros * H_wellformed H_hoare_stmt.
   induction H_hoare_stmt.
-  - repeat lazymatch goal with
-    | H : hoare_lexpr _ _ _ _ |- _ => apply hoare_lexpr_sound in H
-    | H : hoare_expr _ _ _ |- _ => apply hoare_expr_sound with (p := p) in H
-    | H : hoare_write _ _ _ _ |- _ => eapply hoare_write_sound with (p := p) in H
-    end.
-    hnf. intros. inversion H4.
-    + hauto unfold: Hoare.hoare_write, Hoare.hoare_expr, Hoare.hoare_lexpr.
-    + admit. (* assign call rule should be ruled out, but we cnanot prove it now. *)
-    + admit. (* assign call rule should be ruled out, but we cnanot prove it now. *)
-    + unfold Hoare.hoare_lexpr in H0. hauto lq: on.
-(* Qed. *)
-Admitted.
+  - hnf. intros. pinv @exec_stmt.
+    + repeat lazymatch goal with
+      | H : hoare_lexpr _ _ _ _ |- _ => apply hoare_lexpr_sound in H
+      | H : hoare_expr _ _ _ |- _ => apply hoare_expr_sound with (p := p) in H; only 2 : assumption
+      | H : hoare_write _ _ _ _ |- _ => eapply hoare_write_sound with (p := p) in H; only 2 : assumption
+      end.
+      specialize (H0 _ _ _ H4 H15).
+      specialize (H2 _ _ H4 H16); subst v0.
+      eapply exec_write_congruent in H17. 3 : apply H0. 2 : { eapply state_is_valid_field_sound, is_valid_field_sound; eassumption. }
+      specialize (H3 _ _ H4 H17). sfirstorder.
+    + pinv @exec_call; pinv hoare_expr.
+    + pinv @exec_call; pinv hoare_expr.
+    + lazymatch goal with
+      | H : hoare_lexpr _ _ _ _ |- _ => apply hoare_lexpr_sound in H
+      end.
+      unfold ihoare_lexpr in H0. hauto lq: on.
+Qed.
 
 End ConcreteHoare.
- *)
