core/Hoare.v
@@ -1,3 +1,4 @@
+Require Import Coq.ssr.ssrbool.
 Require Import Poulet4.Typed.
 Require Import Poulet4.Syntax.
 Require Import Poulet4.Semantics.
